Intermediate commit

Extraction/Core.lean
@@ -4,40 +4,79 @@ open Lean Meta Elab Term Tactic Grind
 
 namespace Lean.Meta.Grind.Extraction
 
--- Note: Expects `target` to be internalized.
+-- TODO: The extraction mechanism so far is incorrect, as we are not considering equivalent
+--       expressions for subterms. E.g. consider:
+--
+-- example (f g : Nat → Nat) (a b : Nat) (h : g a = b) : f (g a) = 0 := by
+--   grind extract min_ast
+
+-- Note: Expects `target` to be internalized and hash-consed.
 def extractMinAST (target : Expr) : GoalM Expr := do
   foldEqc target target fun node min => do
     let expr := node.self
     if expr.isFalse then return min
     if expr.sizeWithoutSharing < min.sizeWithoutSharing then return expr else return min
 
--- Note: Expects `target` and `e` to be internalized.
-def extractExpr? (target expr : Expr) : GoalM (Option Expr) := do
-  unless expr.hasMVar do
-    if ← isEqv target expr then
-      return expr
-    else
-      return none
-  firstInEqc? target fun e => do
-    -- TODO: We might be careful to reset any assignments performed by isDefEq, as not to hinder the
-    --       possibility of later assignments of sketches' holes.
-    if ← (return !e.isFalse) <&&> isDefEq expr e then
-      return e
-    else
-      return none
+-- Note: Expects `target` to be internalized and hash-consed and `expr` to be hash-consed.
+partial def extractExpr? (target expr : Expr) : GoalM (Option Expr) := do
+  -- TODO: We probably need to check for grind gadgets as well.
+  if expr.isApp then return ← extractApp? target expr
+  match expr with
+  | .mvar _  =>
+    return target
+  | .forallE n dom b i =>
+    firstInEqc? target fun
+      | .forallE _ dom' b' _ => do
+        let some exDom ← extractExpr? dom' dom | return none
+        let some exB ← extractExpr? b' b | return none
+        return some <| .forallE n exDom exB i
+      | _ => return none
+  | .lam n dom b i =>
+    firstInEqc? target fun
+      | .lam _ dom' b' _ => do
+        let some exDom ← extractExpr? dom' dom | return none
+        let some exB ← extractExpr? b' b | return none
+        return some <| .lam n exDom exB i
+      | _ => return none
+  | .lit _ | .const _ _ | .sort _ | .fvar _ | .bvar _ =>
+    let isPresent ← anyInEqc? target (return isSameExpr · expr)
+    if isPresent then return expr else return none
+  | .app .. | .proj .. | .mdata .. | .letE .. =>
+    panic! "reached invalid case in `extractExpr?`"
+where
+  -- Partial applications of functions are not necessarily internalized, so we need to obtain the
+  -- entire application and extract for all arguments "at once".
+  extractApp? (target expr : Expr) : GoalM (Option Expr) := do
+    let fn := expr.getAppFn
+    let args := expr.getAppArgs
+    firstInEqc? target fun e => do
+      unless e.isApp do return none
+      let fn'   := e.getAppFn
+      let args' := e.getAppArgs
+      unless args.size = args'.size do return none
+      let some exFn ← extractExpr? fn' fn | return none
+      let mut exArgs := #[]
+      for arg in args, arg' in args' do
+        let some exArg ← extractExpr? arg' arg | return none
+        exArgs := exArgs.push exArg
+      return some <| mkAppN exFn exArgs
 
 -- Note: This is expected to be run in the context of the failed grind goal, and with `target`
---       being internalized.
-def extract? (target : Expr) : Sketch → GoalM (Option Expr)
-  | .minAST => do
+--       being internalized and hash-consed.
+def extract? (target : Expr) (sketch : Sketch) : GoalM (Option Expr) := do
+  match sketch with
+  | .minAST =>
     extractMinAST target
-  | .expr e => do
+  | .expr e =>
     let e ← shareCommon e
     extractExpr? target e
-  | .or lhs rhs => do
+  | .or lhs rhs =>
     if let some ex ← extract? target lhs then
       return ex
     else
       extract? target rhs
+  | .debug =>
+    forEachEqcRoot fun root => do logInfo m!"{root.self}: {← getEqc root.self}"
+    return none
   | _ =>
     throwError "`grind extract` does not currently support `[]ₛ` or nested (application) sketches"
